\begin{env}[Angular Momentum]
	$$\begin{array}{lll}
			(1)~[\hat{\ell}_{x},\hat{\ell}_{y}] = i\hat{\ell}_{z} & (4)~[\hat{\ell}^{2}, \hat{\ell}_{i}] = 0            & (7)~[\hat{\ell}^{2}, \hat{\ell}_{\pm} ] = 0             \\
			(2)~[\hat{\ell}_{y},\hat{\ell}_{z}] = i\hat{\ell}_{x} & (5)~\hat{\ell}_{\pm} = \ell_{x} \pm i\hat{\ell}_{y} & (8)~[\hat{\ell}_{z}, \hat{\ell}_{\pm}] = \pm \ell_{\pm} \\
			(3)~[\hat{\ell}_{z},\hat{\ell}_{x}] = i\hat{\ell}_{y} & (6)~\hat{\ell}_{+} = \hat{\ell}_{-}^{\dagger}       & (9)~[\hat{\ell}_{+}, \hat{\ell}_{-}]=2\hat{\ell}_{z}
		\end{array}$$
\end{env}

\begin{env}[Spherical Harmonics]
	I need to write up the derivation!
	$$Y_{\ell}^{m}(\theta,\phi) = \sqrt{ \frac{(2\ell+1)(\ell-m)!}{4\pi(\ell+m)!} } e^{im\phi} \mathcal{P}_{\ell}^{m}(\cos\theta)$$
\end{env}

\begin{env}[Radial Equation]
	Derivation!
	$$R_{n\ell}(r) = \sqrt{\left(\frac{2}{na}\right)^3 \frac{(n - \ell - 1)!}{2n(n + \ell)!}} e^{-r/na} \left(\frac{2r}{na}\right)^\ell \left[L_{n-\ell-1}^{2\ell+1}(2r/na)\right]$$

	$$L_{p}^{q}(x)=\frac{x^{-p}e^{x}}{q!}\left( \frac{d}{dx} \right)^{q}(e^{-x}x^{p+q})$$
\end{env}
